Prove generation lemmas

syntax.sig
@@ -3,5 +3,5 @@ nat : Type
 
 Univ : nat -> tm
 Lam : tm -> (bind tm in tm) -> tm
-App : tm -> (bind tm in tm) -> tm -> tm -> tm
+App : (bind tm in tm) -> tm -> tm -> tm
 Pi : tm -> (bind tm in tm) -> tm
